theories/Extraction.v
@@ -25,4 +25,5 @@ Extraction Library Ascii.
 Extraction Library PeanoNat.
 Extraction Library Specif.
 Extraction Library Sumbool.
+Extraction Library monad_utils.
 Extraction Library Ast.
